

Solving Polynomial Equations Using Complex Roots

ZHANG YANG MAT2509036

December 19, 2025



- 1 Fundamental Theorem of Algebra
- 2 Viète Theorem
- 3 Examples of solving Polynomial Equations

Fundamental Theorem of Algebra

Theorem 1

Let $P(z) = a_n z^n + a_{n-1} z^{n-1} + \cdots + a_1 z + a_0$ be a polynomial of degree n with coefficient in \mathbb{C} . Then the polynomial equation $P(z) = 0$ has a root in \mathbb{C} .

Theorem 2

Let $P(z) = a_n z^n + a_{n-1} z^{n-1} + \cdots + a_1 z + a_0$ be a polynomial of degree n with coefficient in \mathbb{C} . Then the polynomial equation $P(z) = 0$ has n roots in \mathbb{C} , counting multiplicities.

Theorem

Theorem 3

Let $P(z)$ be a polynomial of degree n with coefficients in \mathbb{R} . If $\alpha = a + bi$ is a root of $P(z) = 0$ with $b \neq 0$, then $\bar{\alpha} = a - bi$ is also a root of $P(z) = 0$.

Viète Theorem

Theorem

Let z_1, z_2, \dots, z_n be the n roots of the equation $a_n z^n + a_{n-1} z^{n-1} + \dots + a_1 z + a_0 = 0$, where $a_n \neq 0$. Then

$$z_1 + z_2 + \dots + z_n = -\frac{a_{n-1}}{a_n}$$

$$\sum_{1 \leq j < k \leq n} z_j z_k = \frac{a_{n-2}}{a_n}$$

$$\vdots$$

$$\prod_{j=1}^n z_j = (-1)^n \frac{a_0}{a_n}$$

Example 1

Given that $2 - i$ is a root of the equation $z^4 - 3z^2 + az + 40 = 0$, where $a \in \mathbb{R}$. Find the value of a and the other roots of the equation.

Examples

Example 1

Given that $2 - i$ is a root of the equation $z^4 - 3z^2 + az + 40 = 0$, where $a \in \mathbb{R}$. Find the value of a and the other roots of the equation.

Answer

Since $2 - i$ is a root, $2 + i$ is a root.

$$\begin{aligned} P(z) &= [z - (2 - i)][z - (2 + i)]Q(z) \\ &= (z^2 - 4z + 5)Q(z) \\ &= (z^2 - 4z + 5)(z^2 + 4z + 8) + (a + 12)z \\ &= [z - (2 - i)][z - (2 + i)][z - (-2 + i)][z - (-2 - i)] \end{aligned}$$

So $a = -12$ and $z = 2 \pm i, -2 \pm i$

Examples

Example 2

Given that the three roots of the equation $z^3 + 6z^2 + 4z - 3 = 0$ are α, β , and γ . Find $\alpha + \beta + \gamma$.

Answer

Apply the Viète Theorem to get

$$\begin{aligned}\alpha + \beta + \gamma &= -\frac{a_{n-1}}{a_n} \\ &= -\frac{6}{-1} = -6\end{aligned}$$

Solving Polynomial Equations Using Complex Roots

ZHANG YANG MAT2509036

December 19, 2025